src/Language/PlutusIR/Semantics/SemanticEquivalence/CompatibilityLemmas/LetRec.v
@@ -2,6 +2,7 @@ Require Import PlutusCert.Language.PlutusIR.Semantics.Dynamic.
 Require Import PlutusCert.Language.PlutusIR.Semantics.Static.
 Require Import PlutusCert.Language.PlutusIR.Semantics.SemanticEquivalence.LogicalRelation.
 Require Import PlutusCert.Language.PlutusIR.Semantics.SemanticEquivalence.Auto.
+Require Import PlutusCert.Language.PlutusIR.Semantics.SemanticEquivalence.Multisubstitution.Congruence.
 
 Lemma compatibility_LetRec : forall Delta Gamma bs t bs' t' T,
     LR_logically_approximate Delta Gamma (Let Rec bs t) (Let Rec bs' t') T.
